kill some easy admits

src/program_proof/memkv/memkv_marshal_getcid_proof.v
@@ -1,11 +1,12 @@
 From Perennial.program_proof Require Import dist_prelude.
 From Goose.github_com.mit_pdos.gokv Require Import memkv.
+From Perennial.program_proof Require Import marshal_proof.
 From Perennial.program_proof.memkv Require Export common_proof.
 
 Section memkv_marshal_getcid_proof.
 
-Definition has_encoding_Uint64 (data:list u8) (cid:u64) : Prop.
-Admitted.
+Definition has_encoding_Uint64 (data:list u8) (cid:u64) : Prop :=
+  has_encoding data [ EncUInt64 cid ].
 
 Context `{!heapG Σ}.
 
@@ -20,7 +21,30 @@ Lemma wp_encodeUint64 cid :
   }}}
 .
 Proof.
-Admitted.
+  iIntros (Φ) "Hrep HΦ".
+
+  wp_lam.
+  wp_pures.
+  iNamed "Hrep".
+
+  wp_apply (wp_new_enc).
+  iIntros (enc) "Henc".
+  wp_pures.
+
+  wp_apply (wp_Enc__PutInt with "Henc").
+  { word. }
+  iIntros "Henc".
+  wp_pures.
+
+  wp_apply (wp_Enc__Finish with "Henc").
+  iIntros (rep_sl repData).
+  iIntros "(%Henc & %Hlen & Hrep_sl)".
+  iApply "HΦ".
+  iFrame.
+  iPureIntro.
+  rewrite /has_encoding_Uint64.
+  done.
+Qed.
 
 Lemma wp_decodeUint64 sl data cid :
   {{{
@@ -32,6 +56,21 @@ Lemma wp_decodeUint64 sl data cid :
   }}}
 .
 Proof.
-Admitted.
+  iIntros (Φ) "[Hsl %Henc] HΦ".
+  wp_lam.
+  wp_pures.
+
+  iDestruct (typed_slice.is_slice_small_acc with "Hsl") as "[Hsl _]".
+  wp_apply (wp_new_dec with "[$Hsl]").
+  { done. }
+  iIntros (?) "Hdec".
+  wp_pures.
+
+  wp_apply (wp_Dec__GetInt with "[$Hdec]").
+  iIntros "Hdec".
+
+  iApply "HΦ".
+  by iFrame.
+Qed.
 
 End memkv_marshal_getcid_proof.
